$$
d\phi = \frac{1}{4\pi\epsilon_0} \frac{\sigma dS}{R}
$$

$$
\phi = \frac{\sigma a}{2\epsilon_0 l}\left[l + a - \sqrt{a^2 + l^2}\right]
$$

$$
\phi = -\frac{\sigma a}{2\epsilon_0 l}\left[l + a + \sqrt{a^2 + l^2}\right]
$$

$$
\vec{E} = \frac{\sigma a^2}{2\epsilon_0 l^2}\left[1 - \frac{a}{\sqrt{a^2 + l^2}}\right]\hat{k}
$$

$$
\vec{E} = \frac{\sigma a^2}{2\epsilon_0 l^2}\left[ -1 - \frac{a}{\sqrt{a^2 + l^2}}\right]\hat{k}
$$

$$
\vec{E} = -\nabla(\phi)
$$


$$
\vec{F} = \frac{q\sigma a^2}{2\epsilon_0 l^2}\left[1 - \frac{a}{\sqrt{a^2 + l^2}}\right]\hat{k} - mg\hat{k}
$$

$$
\vec{F} = \frac{q\sigma a^2}{2\epsilon_0 l^2}\left[-1 - \frac{a}{\sqrt{a^2 + l^2}}\right]\hat{k} - mg\hat{k}
$$

$$
\vec{E} = \int_{-a}^0 dz \int_{-\sqrt{a^2 - z^2}}^{\sqrt{a^2 - z^2}} dy \int_{-\sqrt{a^2 - z^2 - y^2}}^{\sqrt{a^2 - z^2 - y^2}} dx \frac{\sigma}{4\pi\epsilon_0}\frac{[x_0 - x]\hat{i} + [y_0 - y]\hat{j} + [z_0 - z]\hat{k}}{\left[(x - x_0)^2 + (y - y_0)^2 + (z - z_0)^2  \right]^{3/2}}

$$

$$
\phi = \frac{\sigma}{4\pi\epsilon_0}\int_{-a}^0 dz \int_{-\sqrt{a^2 - z^2}}^{\sqrt{a^2 - z^2}} dy \int_{-\sqrt{a^2 - z^2 - y^2}}^{\sqrt{a^2 - z^2 - y^2}} dx \frac{1}{\left[(x - x_0)^2 + (y - y_0)^2 + (z - z_0)^2  \right]^{1/2}}

$$

$$
\phi = \frac{\sigma a}{2\epsilon_0 l}\left[l + a - \sqrt{a^2 + l^2}\right] + mgl
$$

$$
\phi = -\frac{\sigma a}{2\epsilon_0 l}\left[l + a + \sqrt{a^2 + l^2}\right] + mgl
$$